code/salsa-family/Salsa.fst
@@ -37,21 +37,24 @@ val double_round:
 [@ "c_inline"]
 let double_round st = double_round st
 
+let value_at m (h:HyperStack.mem{live h m}) = reveal_sbytes (as_seq h m)
+
+
 val salsa20:
   output:uint8_p ->
   plain:uint8_p{disjoint output plain} ->
   len:U32.t{U32.v len = length output /\ U32.v len = length plain} ->
   key:uint8_p{length key = 32} ->
-  nonce:uint8_p{length key = 12} ->
+  nonce:uint8_p{length nonce = 8} ->
   ctr:UInt64.t{UInt64.v ctr + (length plain / 64) < pow2 64} ->
   Stack unit
-    (requires (fun h -> live h output /\ live h plain))
-    (ensures (fun h0 _ h1 -> live h1 output /\ live h0 plain
+    (requires (fun h -> live h output /\ live h plain /\ live h key /\ live h nonce))
+    (ensures (fun h0 _ h1 -> live h1 output /\ live h0 plain /\ live h0 key /\ live h0 nonce
       /\ modifies_1 output h0 h1
-      /\ (let o = reveal_sbytes (as_seq h1 output) in
-         let plain = reveal_sbytes (as_seq h0 plain) in
-         let k = reveal_sbytes (as_seq h0 key) in
-         let n = reveal_sbytes (as_seq h0 nonce) in
+      /\ (let o = output `value_at` h1 in
+         let plain = plain `value_at` h0 in
+         let k = key `value_at` h0 in
+         let n = nonce `value_at` h0 in
          let ctr = UInt64.v ctr in
-         o == Spec.CTR.counter_mode Spec.salsa20_ctx Spec.salsa20_cipher k n ctr plain)))
+         o == Spec.Salsa20.salsa20_encrypt_bytes k n ctr plain)))
 let salsa20 output plain len k n ctr = salsa20 output plain len k n ctr
